Refactor interp_prop, new definition

src/coq/Utils/PropT.v
@@ -224,185 +224,35 @@ Section PropMonad.
       ; bind := bind_PropT
     |}.
 
-  (* Definition 5.3: Handler Correctness *)
-  Definition handler_correct {E F} (h_spec: E ~> PropT F) (h: E ~> itree F) :=
-    (forall T e, h_spec T e (h T e)).
-
-  Definition k_spec_correct
-             {E F}
-             (h: E ~> itree F)
-             (k_spec : forall T R, E T -> itree F T -> (T -> itree E R) -> (T -> itree F R) -> itree F R -> Prop) : Prop
-    := forall T R e k1 k2 t2, t2 ≈ bind (h T e) k2 -> k_spec T R e (h T e) k1 k2 t2.
-
-  Inductive interp_PropTF {E F}
-            (h_spec : E ~> PropT F)
-            (k_spec : forall T R, E T -> itree F T -> (T -> itree E R) -> (T -> itree F R) -> itree F R -> Prop)
-            {R : Type} (RR : relation R) (sim : itree E R -> itree F R -> Prop)
-            : itree' E R -> itree F R -> Prop :=
-  | Interp_PropT_Ret : forall r1 r2 (REL: RR r1 r2)
-                     (t2 : itree F R)
-                     (eq2 : t2 ≈ (Ret r2)),
-      interp_PropTF h_spec k_spec RR sim (RetF r1) t2
-
-  | Interp_PropT_Tau : forall t1 t2 (HS: sim t1 t2), interp_PropTF h_spec k_spec RR sim (TauF t1) t2
-                    
-  | Interp_PropT_Vis : forall A (e : E A) (k1 : A -> itree E R)
-                         (t2 : itree F R)
-
-                         (ta :itree F A)
-                         (k2 : A -> itree F R)
-
-                         (HTA: h_spec A e ta)
-                         (HK : forall (a : A), Returns a ta ->  sim (k1 a) (k2 a))
-
-                         (* k_spec => t2 ≈ bind ta k2 *)
-                         (* k_spec => True *)
-                         (KS : k_spec A R e ta k1 k2 t2), 
-      interp_PropTF h_spec k_spec RR sim (VisF e k1) t2.
-
-  Hint Constructors interp_PropTF : core.
-
-  Lemma interp_PropTF_mono E F h_spec k_spec R RR  (t0 : itree' E R) (t1 : itree F R) sim sim'
-        (IN : interp_PropTF h_spec k_spec RR sim t0 t1)
-        (LE : sim <2= sim') : 
-    (interp_PropTF h_spec k_spec RR sim' t0 t1).
+  Lemma Returns_ret_inv_ : forall {E} A (a b : A) (t : itree E A), t ≈ (Ret b) -> Returns a t -> a = b.
   Proof.
-    induction IN; eauto.
+    intros E A a b t eq H.
+    revert b eq.
+    induction H; intros; subst.
+    - rewrite H in eq. apply Eq.eqit_Ret in eq. auto.
+    - eapply IHReturns. rewrite tau_eutt in H. rewrite <- H. assumption.
+    - rewrite H in eq. symmetry in eq. apply eqit_inv in eq; inv eq.
   Qed.
 
-  Hint Resolve interp_PropTF_mono : paco.
-
-  Definition interp_PropT_ E F h_spec k_spec R RR sim (t0 : itree E R) (t1 : itree F R) :=
-    interp_PropTF h_spec k_spec RR sim (observe t0) t1.
-  Hint Unfold interp_PropT_ : core.
-
-  Lemma interp_PropT__mono E F h_spec k_spec R RR : monotone2 (interp_PropT_ E F h_spec k_spec R RR).
-  Proof.
-    do 2 red. intros. eapply interp_PropTF_mono; eauto.
-  Qed.
-  Hint Resolve interp_PropT__mono : paco.
-
-  (* Definition 5.2 *)
-  Definition interp_prop {E F}
-            (h_spec : E ~> PropT F)
-            (k_spec : forall T R, E T -> itree F T -> (T -> itree E R) -> (T -> itree F R) -> itree F R -> Prop)
-    :
-    forall R (RR: relation R), itree E R -> PropT F R :=
-      fun R (RR: relation R) =>  paco2 (interp_PropT_ E F h_spec k_spec R RR) bot2.
-
-  (* Figure 7: Interpreter law for Ret *)
-  Lemma interp_prop_ret :
-    forall R E F
-      (h_spec : E ~> PropT F)
-      (k_spec : forall T R, E T -> itree F T -> (T -> itree E R) -> (T -> itree F R) -> itree F R -> Prop)
-      (r : R)
-    , Eq1_PropT _ (interp_prop h_spec k_spec R eq (ret r)) (ret r).
+  Lemma Returns_ret_inv :  forall {E} A (a b : A), Returns a ((ret b) : itree E A) -> a = b.
   Proof.
     intros.
-    repeat red.
-    split; [| split].
-    - intros. split; intros.
-      + unfold interp_prop in H0.
-        pinversion H0. subst.
-        cbn. rewrite <- H. assumption.
-      + pstep. econstructor. reflexivity. rewrite H. cbn in H0. assumption.
-    - do 3 red.
-      intros t1 t2 eq; split; intros H; pinversion H; subst.
-      + red. pstep. econstructor. reflexivity. rewrite <- eq. assumption.
-      + red. pstep. econstructor. reflexivity. rewrite eq. assumption.
-   - do 3 red. intros. split; intros; cbn in *. rewrite <- H. assumption. rewrite H; assumption.
+    eapply Returns_ret_inv_. reflexivity. cbn in H. apply H.
   Qed.
 
-  #[global] Instance interp_PropTF_Proper
-   {E F}
-   (h_spec : E ~> PropT F)
-   (k_spec : forall T R, E T -> itree F T -> (T -> itree E R) -> (T -> itree F R) -> itree F R -> Prop)
-   R RR (t : itree' E R)
-         (sim : itree E R -> itree F R -> Prop)
-         (HS: forall t, Proper(eutt eq ==> flip impl) (sim t))
-         (KS: forall A R e ta k1 k2, Proper (eutt eq ==> flip impl) (k_spec A R e ta k1 k2))
-    : 
-    Proper(eutt eq ==> iff) (interp_PropTF h_spec k_spec RR sim t).
-  Proof.
-    do 2 red.
-    intros.
-    split; intros.
-    - inversion H0; subst; econstructor; eauto.
-      + rewrite <- H. assumption.
-      + specialize (HS t1). rewrite <- H. assumption.
-      + (* h_spec now depends on the tree `t2`, so we need to show that it respects x ≈ y *)
-        (* Not a guarantee, depends on what h_spec is... So we need a proper instance for that *)
-        rewrite <- H; auto.
-    - inversion H0; subst; econstructor; eauto.
-      rewrite H. assumption. specialize (HS t1). rewrite H. assumption.
-      rewrite H. assumption.
-  Qed.
+  Definition singletonT {E}: itree E ~> PropT E :=
+    fun R t t' => t' ≈ t.
 
-  #[global] Instance interp_prop_Proper
-   {E F}
-   (h_spec : E ~> PropT F)
-   (k_spec : forall T R, E T -> itree F T -> (T -> itree E R) -> (T -> itree F R) -> itree F R -> Prop)
-   R RR (t : itree E R)
-   (KS: forall A R e ta k1 k2, Proper (eutt eq ==> flip impl) (k_spec A R e ta k1 k2)) :
-    Proper(eq_itree Logic.eq ==> iff) (interp_prop h_spec k_spec R RR t).
-  Proof.
-    do 2 red.
-    intros.
-    split.
-    - revert t x y H.
-      pcofix CIH.
-      intros t x y eq HI.
-      red in HI. punfold HI. red in HI.
-      pstep. red. genobs t ot.
-      inversion HI; subst; econstructor; eauto.
-      + rewrite <- eq. assumption.
-      + pclearbot. right. eapply CIH; eauto.
-      + intros. specialize (HK a H0). pclearbot. right. eapply CIH. 2 : { apply HK. } reflexivity.
-      + rewrite <- eq. eauto.
-    - revert t x y H.
-      pcofix CIH.
-      intros t x y eq HI.
-      red in HI. punfold HI. red in HI.
-      pstep. red. genobs t ot.
-      inversion HI; subst; econstructor; eauto.
-      + rewrite eq. assumption.
-      + pclearbot. right. eapply CIH; eauto.
-      + intros. specialize (HK a H0). pclearbot. right. eapply CIH. 2 : { apply HK. } reflexivity.
-      + rewrite eq. eauto.
-  Qed.
+  Definition iter_cont {I E R} (step' : I -> itree E (I + R)) :
+    I + R -> itree E R :=
+    fun lr => ITree.on_left lr l (Tau (ITree.iter step' l)).
 
-  #[global] Instance interp_prop_Proper2
-   {E F}
-   (h_spec : E ~> PropT F)
-   (k_spec : forall T R, E T -> itree F T -> (T -> itree E R) -> (T -> itree F R) -> itree F R -> Prop)
-   R RR (t : itree E R)
-   (KS: forall A R e ta k1 k2, Proper (eutt eq ==> flip impl) (k_spec A R e ta k1 k2)) :
-    Proper(eutt Logic.eq ==> iff) (interp_prop h_spec k_spec R RR t).
-  Proof.
-    do 2 red.
-    intros.
-    split.
-    - revert t x y H.
-      pcofix CIH.
-      intros t x y eq HI.
-      red in HI. punfold HI. red in HI.
-      pstep. red. genobs t ot.
-      inversion HI; subst; econstructor; eauto.
-      + rewrite <- eq. assumption.
-      + pclearbot. right. eapply CIH; eauto.
-      + intros. specialize (HK a H0). pclearbot. right. eapply CIH. 2 : { apply HK. } reflexivity.
-      + rewrite <- eq. eauto.
-    - revert t x y H.
-      pcofix CIH.
-      intros t x y eq HI.
-      red in HI. punfold HI. red in HI.
-      pstep. red. genobs t ot.
-      inversion HI; subst; econstructor; eauto.
-      + rewrite eq. assumption.
-      + pclearbot. right. eapply CIH; eauto.
-      + intros. specialize (HK a H0). pclearbot. right. eapply CIH. 2 : { apply HK. } reflexivity.
-      + rewrite eq. eauto.
-  Qed.
+  #[global] Polymorphic Instance MonadIter_Prop {E} : MonadIter (PropT E) :=
+    fun R I (step : I -> PropT E (I + R)) i =>
+      fun (r : itree E R) =>
+        (exists (step' : I -> (itree E (I + R)%type)),
+                ITree.bind (step' i) (@iter_cont I E R step') ≈ r /\
+                (forall j, step j (step' j))).
 
   (* This exists in the stdlib as [ProofIrrelevance.inj_pair2], but we reprove
    it to not depend on proof irrelevance (we use axiom [JMeq.JMeq_eq] instead).
@@ -420,303 +270,34 @@ Section PropMonad.
         end).
   Qed.
 
-  (* TODO: Move this *)
-  Lemma eqit_flip_symmetric {E R} (RR : R -> R -> Prop) `{Symmetric R RR} b1 b2:
-    forall (u : itree E R) (v : itree E R),
-      eqit RR b1 b2 u v -> eqit (flip RR) b1 b2 u v.
+  Lemma eqit_bind_Returns_inv {E} {R S T} (RS : R -> S -> Prop)
+        (t : itree E T)  (k1: T -> itree E R) (k2 : T -> itree E S) :
+    (eutt RS  (ITree.bind t k1) (ITree.bind t k2)) ->
+    (forall r, Returns r t -> eutt RS (k1 r) (k2 r)).
   Proof.
-    pcofix self; pstep. intros u v euv. punfold euv.
-    red in euv |- *. induction euv; pclearbot; eauto 7 with paco.
-  Qed.
-
-  #[global] Instance interp_prop_Proper3
-   {E F} {a b}
-   (h_spec : E ~> PropT F)
-   (k_spec : forall T R, E T -> itree F T -> (T -> itree E R) -> (T -> itree F R) -> itree F R -> Prop)
-   (KP : forall T R RR b a, Proper (eq ==> eq ==> (fun k1 k2 => forall x, eqit RR b a (k1 x) (k2 x)) ==> eq ==> eq ==> iff) (k_spec T R))
-   R RR :
-    Proper(eqit eq a b ==> eq  ==> iff) (interp_prop h_spec k_spec R RR).
-  Proof.
-    do 4 red.
-    intros; split.
-    - subst.
-      revert x y H y0.
-      pcofix CIH.
-      intros x y eq t H.
-      pstep; red.
-      punfold H. red in H.
-
-      punfold eq. red in eq.
-      genobs x obsx.
-      genobs y obsy.
-      revert x y Heqobsx Heqobsy t H.
-
-      induction eq; intros x y Heqobsx Heqobsy t H; inversion H; subst; pclearbot.
-      + econstructor; eauto.
-      + econstructor. right. eapply CIH. apply REL. apply HS.
-      + apply inj_pair2 in H2.
-        apply inj_pair2 in H3. subst.
-        econstructor; eauto. intros X HX. specialize (REL X). specialize (HK X HX). pclearbot.
-        right.
-
-        eapply CIH; eauto.
-        eapply KP; eauto.
-        intros.
-        eapply eqit_flip;
-        eapply eqit_flip_symmetric; eauto; typeclasses eauto.
-      + eapply IHeq.  reflexivity. reflexivity.
-        punfold HS.
-      + econstructor. left. pstep. eapply IHeq. reflexivity. reflexivity. assumption.
-      + econstructor. left.  pstep. eapply IHeq. reflexivity. reflexivity. assumption.
-      + econstructor. left.  pstep. eapply IHeq. reflexivity. reflexivity. assumption.
-
-   - subst.
-      revert x y H y0.
-      pcofix CIH.
-      intros x y eq t H.
-      pstep; red.
-      punfold H. red in H.
-
-      punfold eq. red in eq.
-      genobs x obsx.
-      genobs y obsy.
-      revert x y Heqobsx Heqobsy t H.
-
-      induction eq; intros x y Heqobsx Heqobsy t H; inversion H; subst; pclearbot.
-      + econstructor; eauto.
-      + econstructor. right. eapply CIH. apply REL. apply HS.
-      + apply inj_pair2 in H2.
-        apply inj_pair2 in H3. subst.
-        econstructor; eauto. intros X HX. specialize (REL X). specialize (HK X HX). pclearbot.
-        right.
-
-        eapply CIH; eauto.
-        eapply KP; eauto.
-      + econstructor. left. pstep. eapply IHeq. reflexivity. reflexivity. assumption.
-      + econstructor. left. pstep. eapply IHeq. reflexivity. reflexivity. assumption.
-      + econstructor. left. pstep. eapply IHeq. reflexivity. reflexivity. assumption.
-      + eapply IHeq. reflexivity. reflexivity.   punfold HS.
-  Qed.
-
-    Lemma interp_prop_ret_pure :
-      forall {T E F} (RR : relation T) `{REF: Reflexive _ RR} (x : T)
-        (h : E ~> PropT F)
-        (k_spec : forall T R, E T -> itree F T -> (T -> itree E R) -> (T -> itree F R) -> itree F R -> Prop),
-      interp_prop h k_spec _ RR (ret x) (ret x).
-    Proof.
-      intros T E F RR REF x h k_spec.
-      generalize dependent x.
-      pcofix CIH.
-      intros x.
-      pstep.
-      cbn.
-      econstructor.
-      reflexivity.
-      reflexivity.
-    Qed.
- 
-    Lemma interp_prop_ret_refine :
-      forall {T E F} (RR : relation T) (x y : T)
-        (h : E ~> PropT F)
-        (k_spec : forall T R, E T -> itree F T -> (T -> itree E R) -> (T -> itree F R) -> itree F R -> Prop),
-        RR x y ->
-        interp_prop h k_spec _ RR (ret x) (ret y).
-    Proof.
-      intros T E F RR x y h k_spec RRxy.
-      generalize dependent y.
-      generalize dependent x.
-      pcofix CIH.
-      intros x y RRxy.
-      pstep.
-      cbn.
-      econstructor; eauto.
-      reflexivity.
-    Qed.
-
-    Lemma interp_prop_refl_h :
-      forall {T E} (RR : relation T) `{REF: Reflexive _ RR} (t1 t2 : itree E T)
-        (h : E ~> PropT E)
-        (k_spec : forall T R, E T -> itree E T -> (T -> itree E R) -> (T -> itree E R) -> itree E R -> Prop),
-        (forall {X : Type} (e : E X), h X e (trigger e)) ->
-        (k_spec_correct (fun T e => trigger e) k_spec) ->
-        t1 ≈ t2 ->
-        interp_prop h k_spec _ RR t1 t2.
-    Proof.
-      intros T E RR REF t1 t2 h k_spec H_SPEC K_SPEC EQ.
-      generalize dependent t2.
-      generalize dependent t1.
-      pcofix CIH.
-      intros t1 t2 EQ.
-      pose proof (itree_eta t1) as ETA.
-      destruct (observe t1) eqn:Ht1.
-      - pstep.
-        red.
-        rewrite Ht1.
-        econstructor.
-        reflexivity.
-        rewrite <- EQ.
-        rewrite ETA.
-        reflexivity.
-      - pstep.
-        red.
-        rewrite Ht1.
-        econstructor.
-        right.
-        apply CIH; auto.
-        rewrite <- tau_eutt.
-        rewrite <- ETA.
-        auto.
-      - pstep.
-        red.
-        rewrite Ht1.
-        eapply Interp_PropT_Vis with (k2 := k).
-        + eauto.
-        + intros a RET.
-          right.
-          apply CIH.
-          reflexivity.
-        + eapply K_SPEC. rewrite <- EQ.
-          setoid_rewrite bind_trigger.
-          cbn.
-          rewrite ETA.
-          reflexivity.
-    Qed.
-
-    Lemma interp_prop_refl :
-      forall {T E} (RR : relation T) `{REF: Reflexive _ RR} (t : itree E T)
-        (h : forall X : Type, E X -> PropT E X)
-        (k_spec : forall T R, E T -> itree E T -> (T -> itree E R) -> (T -> itree E R) -> itree E R -> Prop),
-        (forall {X : Type} (e : E X), h X e (trigger e)) ->
-        (k_spec_correct (fun T e => trigger e) k_spec) ->
-        interp_prop h k_spec _ RR t t.
-    Proof.
-      intros T E RR REF t h k_spec H_SPEC K_SPEC.
-      apply interp_prop_refl_h; eauto.
-      reflexivity.
-    Qed.
-
-  (* Lemma 5.4: interp_prop_correct - note that the paper presents a slightly simpler formulation where t = t' *)
-  Lemma interp_prop_correct_exec:
-    forall {E F}
-      (h_spec : E ~> PropT F)
-      (k_spec : forall T R, E T -> itree F T -> (T -> itree E R) -> (T -> itree F R) -> itree F R -> Prop)
-      (h: E ~> itree F)
-      (HC : handler_correct h_spec h)
-      (KC : k_spec_correct h k_spec),
-      forall R RR `{Reflexive _ RR} t t', t ≈ t' -> interp_prop h_spec k_spec R RR t (interp h t').
-  Proof.
-    intros E F h_spec k_spec h HC KC R RR H t t' H1.
-    revert t t' H1.
-    pcofix CIH.
-    intros t t' eq.
-    pstep.
-    red.
-    unfold interp, Basics.iter, MonadIter_itree.
-    rewrite (itree_eta t) in eq.
-    destruct (observe t).
-    - econstructor. reflexivity. rewrite <- eq. rewrite unfold_iter. cbn. rewrite Eq.bind_ret_l. cbn.  reflexivity.
-    - econstructor. right.
-      eapply CIH. rewrite tau_eutt in eq. rewrite eq. reflexivity.
-    - econstructor.
-      apply HC.
-      intros a. cbn.  
-      right.
-      unfold interp, Basics.iter, MonadIter_itree in CIH. unfold fmap, Functor_itree, ITree.map in CIH.
-      specialize (CIH (k a) (k a)).
-      apply CIH.
-      reflexivity.
-
-      unfold k_spec_correct in KC.
-      
-      eapply KC.
-      rewrite <- eq.
-      rewrite unfold_iter.
-      cbn.
-
-      rewrite bind_map.
-      eapply eutt_clo_bind.
-      reflexivity.
-      intros u1 u2 H0; subst.
-
-      rewrite tau_eutt.
-      reflexivity.
-  Qed.
-
-  (* Lemma 5.5 - note that the paper presents this lemma after unfolding the definition of Proper.
-   *)
-  Instance interp_prop_Proper_eq :
-    forall R (RR : relation R) (HR: Reflexive RR) (HT : Transitive RR) E F
-      (h_spec : E ~> PropT F)
-      (k_spec : forall T R, E T -> itree F T -> (T -> itree E R) -> (T -> itree F R) -> itree F R -> Prop)
-      (KP : forall T R RR b a, Proper (eq ==> eq ==> (fun k1 k2 => forall x, eqit RR b a (k1 x) (k2 x)) ==> eq ==> eq ==> iff) (k_spec T R)),
-      Proper (@eutt _ _ _ RR ==> eq ==> flip Basics.impl) (@interp_prop E _ h_spec k_spec R RR).
-  Proof.
-    intros.
-
-    do 5 red.
-    intros t1 t2 eqt s' s eqs HI.
-    subst.
-
-    revert t1 t2 eqt s HI.
-
-    pcofix CIH.
-
-    intros.
-
-    pstep. red.
-    punfold HI. red in HI.
-
-    punfold eqt. red in eqt.
-    genobs t1 obst1.
-    genobs t2 obst2.
-    revert t1 t2 Heqobst1 Heqobst2 s HI.
-
-    induction eqt; intros.
-    - inversion HI; subst.
-      econstructor. etransitivity; eauto. assumption.
-    - inversion HI; subst.
-      econstructor. pclearbot. right.  eapply CIH; eauto.
-    - inversion HI.
-      subst.
-      apply inj_pair2 in H1.
+    intros EQIT r HRET.
+    revert R S RS k1 k2 EQIT.
+    induction HRET; intros.
+    - rewrite H in EQIT.
+      do 2 rewrite Eq.bind_ret_l in EQIT.
+      assumption.
+    - rewrite tau_eutt in H. rewrite H in EQIT.
+      eapply IHHRET; eauto.
+    - rewrite H in EQIT.
+      do 2 rewrite Eq.bind_vis in EQIT.
+      repeat red in EQIT. punfold EQIT.
+      inversion EQIT.
       apply inj_pair2 in H2.
+      apply inj_pair2 in H3.
+      apply inj_pair2 in H4.
+      apply inj_pair2 in H5.
       subst.
-      econstructor.
-      apply HTA.
-      intros a Ha. specialize (REL a). specialize (HK a Ha). red in REL. pclearbot.
-      right. eapply CIH. apply REL. apply HK.
-      eapply KP; eauto.
+      eapply IHHRET.
+      specialize (REL x).
+      red in REL.
       pclearbot.
-      intros x.
-      eapply REL.
-    - econstructor.
-      left. pstep. red. eapply IHeqt. reflexivity. eassumption. assumption.
-    - inversion HI; subst.
-      pclearbot.
-      eapply IHeqt. reflexivity. reflexivity.
-      pinversion HS.
+      apply REL.
   Qed.
-
-    Lemma interp_prop_trans :
-      forall {T E} (RR : relation T) `{REF: Reflexive _ RR} `{TRANS: Transitive _ RR} (x y z : itree E T)
-        (h : forall X : Type, E X -> PropT E X)
-        (k_spec : forall T R, E T -> itree E T -> (T -> itree E R) -> (T -> itree E R) -> itree E R -> Prop),
-        (forall {X : Type} (e : E X), h X e (trigger e)) ->
-        (k_spec_correct (fun T e => trigger e) k_spec) ->
-        interp_prop h k_spec _ RR x y ->
-        interp_prop h k_spec _ RR y z ->
-        interp_prop h k_spec _ RR x z.
-    Proof.
-      intros T E RR REF TRANS x y z h k_spec H_SPEC K_SPEC XY YZ.
-      revert x y z XY YZ.
-      pcofix CIH; intros x y z XY YZ.
-
-      punfold XY; punfold YZ; pfold; red in XY, YZ |- *.
-      genobs x xo.
-      genobs y yo.
-      genobs z zo.
-    Abort.
-
 
   #[global] Instance Returns_eutt {E A} a: Proper (eutt eq ==> iff) (@Returns E A a).
   Proof.
@@ -761,291 +342,6 @@ Section PropMonad.
   Proof.
     intros.
     apply eutt_Returns_. auto.
-  Qed.
-
-  (* Figure 7: interp Trigger law *)
-  (* morally, we should only work with "proper" triggers everywhere *)
-  (* Lemma interp_prop_trigger : *)
-  (*   forall E F *)
-  (*     (h_spec : E ~> PropT F) *)
-  (*     R (e : E R) *)
-  (*     (HP : forall T R k t2, Proper (eq ==> Eq1_PropT T) (fun e ift => h_spec T R e ift k t2)) *)
-  (*   , (forall k t2, Eq1_PropT _ (interp_prop h_spec k_spec R eq (trigger e)) (fun ifr => h_spec R R R e ifr k t2)). *)
-  (* Proof. *)
-  (*   intros. *)
-  (*   red. *)
-  (*   split; [| split]. *)
-  (*   - intros; split; intros. *)
-  (*     + unfold trigger in H0. red in H0. *)
-  (*       pinversion H0; subst. *)
-  (*       apply inj_pair2 in H3. apply inj_pair2 in H4. *)
-  (*       subst. *)
-  (*       unfold subevent, resum, ReSum_id, Id_IFun, id_ in HTA. *)
-  (*       rewrite eq2 in H. *)
-  (*       assert (x <- ta ;; k2 x ≈ ta). *)
-  (*       { rewrite <- (Eq.bind_ret_r ta). *)
-  (*         apply eutt_clo_bind with (UU := fun u1 u2 => u1 = u2 /\ Returns u1 ta). *)
-  (*         rewrite Eq.bind_ret_r. apply eutt_Returns. *)
-  (*         intros. destruct H1. subst. specialize (HK u2 H2). pclearbot. pinversion HK. subst. assumption. *)
-  (*       } *)
-  (*       rewrite H1 in H. *)
-  (*       specialize (HP R e e eq_refl).  unfold Eq1_PropT in HP. destruct HP as (P & _ & _). *)
-  (*       rewrite P. apply HTA. symmetry. assumption. *)
-  (*     + unfold trigger, subevent, resum, ReSum_id, Id_IFun, id_. *)
-  (*       red. pstep. eapply Interp_PropT_Vis with (k2 := (fun x : R => Ret x)). *)
-  (*       * apply H0. *)
-  (*       * unfold bind, Monad_itree. rewrite Eq.bind_ret_r. assumption. *)
-  (*       * intros a. left. pstep. red. econstructor. reflexivity.  reflexivity. *)
-  (*   - do 4 red. intros; split; intros. *)
-  (*     rewrite <- H. assumption. *)
-  (*     rewrite H. assumption. *)
-  (*   - do 4 red. *)
-  (*     intros; split; intros. *)
-  (*     specialize (HP R e e eq_refl). destruct HP as (P & _ & _). *)
-  (*     rewrite P; eauto. symmetry. assumption. *)
-  (*     specialize (HP R e e eq_refl). destruct HP as (P & _ & _). *)
-  (*     rewrite P; eauto.  *)
-  (* Qed. *)
-
-  (*  Interesting observations about interp_prop:
-
-      Suppose h_spec : E ~> Prop T F
-      then (interp_prop h_spec k_spec _ eq spin) : PropT F
-      which itrees should be accepted by that predicate?  
-     
-      - we know by interp_prop_correct_exe that if there is an h such that handler_correct h_spec h then spin is accepted.
-        (I believe we could eliminate the requirement that there is such an h)
-      - what other trees are accepted?
-
-      Answer: all of them!
-   *)
-  Lemma interp_prop_spin_accepts_anything :
-    forall E F
-      (h_spec : E ~> PropT F)
-      (k_spec : forall T R, E T -> itree F T -> (T -> itree E R) -> (T -> itree F R) -> itree F R -> Prop)
-      R RR (t : itree F R),
-      interp_prop h_spec k_spec R RR ITree.spin t.
-  Proof.
-    intros.
-    pcofix CIH.
-    pstep. red. cbn. econstructor. right. apply CIH.
-  Qed.
-
-  (* Figure 7: Structural law for tau *)
-  Lemma interp_prop_tau :
-    forall E F
-      (h_spec : E ~> PropT F)
-      (k_spec : forall T R, E T -> itree F T -> (T -> itree E R) -> (T -> itree F R) -> itree F R -> Prop)
-      R RR
-      (t_spec : itree E R)
-      (KP : forall T R e t k1 k2, Proper (eutt eq ==> flip impl) (k_spec T R e t k1 k2)),
-      Eq1_PropT _ (interp_prop h_spec k_spec R RR t_spec) (interp_prop h_spec k_spec R RR (Tau t_spec)).
-  Proof.
-    intros.
-    split; [| split].
-    - intros; split; intros.
-      + rewrite <- H.
-        pstep. red. econstructor. left.
-        apply H0.
-      + rewrite H.
-        pinversion H0. subst.
-        apply HS.
-    - red. typeclasses eauto.
-    - red. typeclasses eauto.
-  Qed.
-
-  Lemma interp_prop_ret_inv :
-    forall E F
-      (h_spec : E ~> PropT F)
-      (k_spec : forall T R, E T -> itree F T -> (T -> itree E R) -> (T -> itree F R) -> itree F R -> Prop)
-      R RR
-      (r1 : R)
-      (t : itree F R)
-      (H : interp_prop h_spec k_spec R RR (ret r1) t),
-       exists  r2, RR r1 r2 /\ t ≈ ret r2.
-  Proof.
-    intros.
-    punfold H.
-    red in H. inversion H; subst.
-    exists r2; eauto.
-  Qed.
-
-  Lemma interp_prop_vis_inv :
-    forall E F
-      (h_spec : E ~> PropT F)
-      (k_spec : forall T R, E T -> itree F T -> (T -> itree E R) -> (T -> itree F R) -> itree F R -> Prop)
-      R RR S
-      (e : E S)
-      (k : S -> itree E R)
-      (t : itree F R)
-      (H : interp_prop h_spec k_spec R RR (vis e k) t), 
-    exists  ms, exists (ks : S -> itree F R),
-      h_spec S e ms /\ k_spec S R e ms k ks t.
-  Proof.
-    intros.
-    punfold H.
-    red in H. inversion H; subst.
-    apply inj_pair2 in H2.
-    apply inj_pair2 in H3.
-    subst.
-    exists ta. exists k2. auto.
-  Qed.
-
-  Lemma interp_prop_tau_inv :
-    forall E F
-      (h_spec : E ~> PropT F)
-      (k_spec : forall T R, E T -> itree F T -> (T -> itree E R) -> (T -> itree F R) -> itree F R -> Prop)
-      R RR 
-      (s : itree E R)
-      (t : itree F R)
-      (H : interp_prop h_spec k_spec R RR (Tau s) t), 
-      interp_prop h_spec k_spec R RR s t.
-  Proof.
-    intros.
-    punfold H.
-    red in H. inversion H; subst.
-    pclearbot.
-    apply HS.
-  Qed.
-
-  Lemma Returns_ret_inv_ : forall {E} A (a b : A) (t : itree E A), t ≈ (Ret b) -> Returns a t -> a = b.
-  Proof.
-    intros E A a b t eq H.
-    revert b eq.
-    induction H; intros; subst.
-    - rewrite H in eq. apply Eq.eqit_Ret in eq. auto.
-    - eapply IHReturns. rewrite tau_eutt in H. rewrite <- H. assumption.
-    - rewrite H in eq. symmetry in eq. apply eqit_inv in eq; inv eq.
-  Qed.
-
-  Lemma Returns_ret_inv :  forall {E} A (a b : A), Returns a ((ret b) : itree E A) -> a = b.
-  Proof.
-    intros.
-    eapply Returns_ret_inv_. reflexivity. cbn in H. apply H.
-  Qed.
-  Lemma case_prop_handler_correct:
-    forall {E1 E2 F}
-      (h1_spec: E1 ~> PropT F)
-      (h2_spec: E2 ~> PropT F)
-      (h1: E1 ~> itree F)
-      (h2: E2 ~> itree F)
-      (C1: handler_correct h1_spec h1)
-      (C2: handler_correct h2_spec h2),
-      handler_correct (case_ h1_spec h2_spec) (case_ h1 h2).
-  Proof.
-    intros E1 E2 F h1_spec h2_spec h1 h2 C1 C2.
-    unfold handler_correct in *.
-    intros T e.
-    destruct e. apply C1. apply C2.
-  Qed.
-
-  (*
-  Lemma case_prop_handler_correct:
-    forall {E1 E2 F}
-      (h1_spec: E1 ~> PropT F)
-      (h2_spec: E2 ~> PropT F)
-      (h1: E1 ~> itree F)
-      (h2: E2 ~> itree F)
-      (C1: handler_correct h1_spec h1)
-      (C2: handler_correct h2_spec h2),
-      handler_correct (case_ h1_spec h2_spec) (case_ h1 h2).
-  Proof.
-    intros E1 E2 F h1_spec h2_spec h1 h2 C1 C2.
-    unfold handler_correct in *.
-    intros T e.
-    destruct e. apply C1. apply C2.
-  Qed.
-*)
-
-  (*
-  Lemma case_prop_handler_correct:
-    forall {E1 E2 F}
-      (h1_spec : forall T R, E1 T -> itree F T -> (T -> itree F R) -> itree F R -> Prop)
-      (h2_spec : forall T R, E2 T -> itree F T -> (T -> itree F R) -> itree F R -> Prop)
-      (h1: E1 ~> itree F)
-      (h2: E2 ~> itree F)
-      (C1: handler_correct h1_spec h1)
-      (C2: handler_correct h2_spec h2),
-      handler_correct
-        (fun (T R : Type)
-           e12
-           ta
-           k
-           t2
-         =>
-           ((case_
-              ((fun (e : E1 T) (t : itree F T) => h1_spec T R e t k t2) : E1 T -> itree F T -> Prop)
-              ((fun (e : E2 T) (t : itree F T) => h2_spec T R e t k t2) : E2 T -> itree F T -> Prop)) _ e12 ta))
-        (case_ h1 h2).
-  Proof.
-    intros E1 E2 F h1_spec h2_spec h1 h2 C1 C2.
-    unfold handler_correct in *.
-    intros T R e k t2.
-    destruct e. apply C1. apply C2.
-  Qed.
- *)
-
-  Definition prop_compose :=
-    fun {F G : Type -> Type } {T : Type} (TT : relation T)
-      (g_spec : F ~> PropT G)
-      (k_spec : forall T R : Type, F T -> itree G T -> (T -> itree F R) -> (T -> itree G R) -> itree G R -> Prop)
-      (PF: PropT F T) (g:itree G T) =>
-      exists f : itree F T, PF f /\ (interp_prop g_spec k_spec) T TT f g.
-
-  (* I don't understand this... *)
-  (* Definition handler_correct_prop *)
-  (*            {E F G} *)
-  (*            (h_spec : E ~> PropT F) *)
-  (*            (h: E ~> itree F) *)
-  (*            (g_spec : forall T R , F T -> itree G T -> (A -> itree G R) -> itree G R -> Prop) *)
-  (*            (g: F ~> itree G) *)
-  (*   := *)
-  (*     (forall T TT e, *)
-  (*         (prop_compose TT g_spec (fun ift => h_spec _ T _ e ift)) *)
-  (*           (interp g (h T e))). *)
-
-
-  Definition singletonT {E}: itree E ~> PropT E :=
-    fun R t t' => t' ≈ t.
-
-  Definition iter_cont {I E R} (step' : I -> itree E (I + R)) :
-    I + R -> itree E R :=
-    fun lr => ITree.on_left lr l (Tau (ITree.iter step' l)).
-
-  #[global] Polymorphic Instance MonadIter_Prop {E} : MonadIter (PropT E) :=
-    fun R I (step : I -> PropT E (I + R)) i =>
-      fun (r : itree E R) =>
-        (exists (step' : I -> (itree E (I + R)%type)),
-                ITree.bind (step' i) (@iter_cont I E R step') ≈ r /\
-                (forall j, step j (step' j))).
-
-  Lemma eqit_bind_Returns_inv {E} {R S T} (RS : R -> S -> Prop)
-        (t : itree E T)  (k1: T -> itree E R) (k2 : T -> itree E S) :
-    (eutt RS  (ITree.bind t k1) (ITree.bind t k2)) ->
-    (forall r, Returns r t -> eutt RS (k1 r) (k2 r)).
-  Proof.
-    intros EQIT r HRET.
-    revert R S RS k1 k2 EQIT.
-    induction HRET; intros.
-    - rewrite H in EQIT.
-      do 2 rewrite Eq.bind_ret_l in EQIT.
-      assumption.
-    - rewrite tau_eutt in H. rewrite H in EQIT.
-      eapply IHHRET; eauto.
-    - rewrite H in EQIT.
-      do 2 rewrite Eq.bind_vis in EQIT.
-      repeat red in EQIT. punfold EQIT.
-      inversion EQIT.
-      apply inj_pair2 in H2.
-      apply inj_pair2 in H3.
-      apply inj_pair2 in H4.
-      apply inj_pair2 in H5.
-      subst.
-      eapply IHHRET.
-      specialize (REL x).
-      red in REL.
-      pclearbot.
-      apply REL.
   Qed.
 
   Section ReturnsBind.
@@ -1845,7 +1141,6 @@ Module BIND_BIND_COUNTEREXAMPLE.
 Qed.
 
 Lemma bind_bind_counterexample:
-      (* eutt_closed PA -> *)
     exists t, bind PA (fun a => bind (KB a) KC) t /\ ~ (bind (bind PA KB) KC t).
 Proof.
   exists t.
