src/coq/Utils/InterpProp.v
@@ -1,0 +1,668 @@
+(* begin hide *)
+From ITree Require Import
+     ITree
+     ITreeFacts
+     Basics.HeterogeneousRelations
+     Events.State
+     Events.StateFacts
+     InterpFacts
+     KTreeFacts
+     Core.ITreeMonad
+     CategoryKleisli
+     CategoryKleisliFacts
+     Eq.Eq.
+
+From ExtLib Require Import
+     Structures.Functor.
+
+From Coq Require Import
+     RelationClasses
+     Strings.String
+     Logic
+     Morphisms
+     Relations
+     List
+     Program.Tactics.
+
+From ITree Require Import
+     Basics.Monad
+     Basics.MonadState.
+
+From Vellvm Require Import
+     Utils.PropT.
+Require Import Paco.paco.
+
+Import ListNotations.
+Import ITree.Basics.Basics.Monads.
+
+
+Import MonadNotation.
+Import CatNotations.
+Local Open Scope monad_scope.
+Local Open Scope cat_scope.
+(* end hide *)
+
+Section interp_prop.
+
+  (* Definition 5.3: Handler Correctness *)
+  Definition handler_correct {E F} (h_spec: E ~> PropT F) (h: E ~> itree F) :=
+    (forall T e, h_spec T e (h T e)).
+
+  Lemma case_prop_handler_correct:
+    forall {E1 E2 F}
+      (h1_spec: E1 ~> PropT F)
+      (h2_spec: E2 ~> PropT F)
+      (h1: E1 ~> itree F)
+      (h2: E2 ~> itree F)
+      (C1: handler_correct h1_spec h1)
+      (C2: handler_correct h2_spec h2),
+      handler_correct (case_ h1_spec h2_spec) (case_ h1 h2).
+  Proof.
+    intros E1 E2 F h1_spec h2_spec h1 h2 C1 C2.
+    unfold handler_correct in *.
+    intros T e.
+    destruct e. apply C1. apply C2.
+  Qed.
+
+  Definition k_spec_correct
+             {E F}
+             (h: E ~> itree F)
+             (k_spec : forall T R, E T -> itree F T -> (T -> itree E R) -> (T -> itree F R) -> itree F R -> Prop) : Prop
+    := forall T R e k1 k2 t2, t2 ≈ bind (h T e) k2 -> k_spec T R e (h T e) k1 k2 t2.
+
+  Inductive interp_PropTF {E F}
+            (h_spec : E ~> PropT F)
+            (k_spec : forall T R, E T -> itree F T -> (T -> itree E R) -> (T -> itree F R) -> itree F R -> Prop)
+            {R : Type} (RR : relation R) (sim : itree E R -> itree F R -> Prop)
+            : itree' E R -> itree F R -> Prop :=
+  | Interp_PropT_Ret : forall r1 r2 (REL: RR r1 r2),
+      interp_PropTF h_spec k_spec RR sim (RetF r1) (Ret r2)
+
+  | Interp_PropT_Tau : forall t1 t2 (HS: sim t1 t2),
+      interp_PropTF h_spec k_spec RR sim (TauF t1) (Tau t2)
+
+  | Interp_PropT_TauP : forall t1 t2 (HS: interp_PropTF h_spec k_spec RR sim (observe t1) t2),
+      interp_PropTF h_spec k_spec RR sim (TauF t1) t2
+
+  | Interp_PropT_Vis : forall A (e : E A) (k1 : A -> itree E R)
+                         (t2 : itree F R)
+
+                         (ta :itree F A)
+                         (k2 : A -> itree F R)
+
+                         (HTA: h_spec A e ta)
+                         (HK : forall (a : A), Returns a ta ->  sim (k1 a) (k2 a))
+
+                         (* k_spec => t2 ≈ bind ta k2 *)
+                         (* k_spec => True *)
+                         (KS : k_spec A R e ta k1 k2 t2), 
+      interp_PropTF h_spec k_spec RR sim (VisF e k1) t2.
+
+  Hint Constructors interp_PropTF : core.
+
+  Lemma interp_PropTF_mono E F h_spec k_spec R RR  (t0 : itree' E R) (t1 : itree F R) sim sim'
+        (IN : interp_PropTF h_spec k_spec RR sim t0 t1)
+        (LE : sim <2= sim') : 
+    (interp_PropTF h_spec k_spec RR sim' t0 t1).
+  Proof.
+    induction IN; eauto.
+  Qed.
+
+  Hint Resolve interp_PropTF_mono : paco.
+
+  Definition interp_PropT_ E F h_spec k_spec R RR sim (t0 : itree E R) (t1 : itree F R) :=
+    interp_PropTF h_spec k_spec RR sim (observe t0) t1.
+  Hint Unfold interp_PropT_ : core.
+
+  Lemma interp_PropT__mono E F h_spec k_spec R RR : monotone2 (interp_PropT_ E F h_spec k_spec R RR).
+  Proof.
+    do 2 red. intros. eapply interp_PropTF_mono; eauto.
+  Qed.
+  Hint Resolve interp_PropT__mono : paco.
+
+  (* Definition 5.2 *)
+  Definition interp_prop {E F}
+            (h_spec : E ~> PropT F)
+            (k_spec : forall T R, E T -> itree F T -> (T -> itree E R) -> (T -> itree F R) -> itree F R -> Prop)
+    :
+    forall R (RR: relation R), itree E R -> PropT F R :=
+      fun R (RR: relation R) =>  paco2 (interp_PropT_ E F h_spec k_spec R RR) bot2.
+
+  (* #[global] Instance interp_PropTF_Proper *)
+  (*  {E F} *)
+  (*  (h_spec : E ~> PropT F) *)
+  (*  (k_spec : forall T R, E T -> itree F T -> (T -> itree E R) -> (T -> itree F R) -> itree F R -> Prop) *)
+  (*  R RR (t : itree' E R) *)
+  (*        (sim : itree E R -> itree F R -> Prop) *)
+  (*        (HS: forall t, Proper(eutt eq ==> flip impl) (sim t)) *)
+  (*        (KS: forall A R e ta k1 k2, Proper (eutt eq ==> flip impl) (k_spec A R e ta k1 k2)) *)
+  (*   :  *)
+  (*   Proper(eutt eq ==> iff) (interp_PropTF h_spec k_spec RR sim t). *)
+  (* Proof. *)
+  (*   do 2 red. *)
+  (*   intros. *)
+  (*   split; intros. *)
+  (*   - inversion H0; subst; econstructor; eauto. *)
+  (*     + rewrite <- H. assumption. *)
+  (*     + specialize (HS t1). rewrite <- H. assumption. *)
+  (*     + (* h_spec now depends on the tree `t2`, so we need to show that it respects x ≈ y *) *)
+  (*       (* Not a guarantee, depends on what h_spec is... So we need a proper instance for that *) *)
+  (*       rewrite <- H; auto. *)
+  (*   - inversion H0; subst; econstructor; eauto. *)
+  (*     rewrite H. assumption. specialize (HS t1). rewrite H. assumption. *)
+  (*     rewrite H. assumption. *)
+  (* Qed. *)
+  (* Figure 7: Interpreter law for Ret *)
+  Lemma interp_prop_ret :
+    forall R E F
+      (h_spec : E ~> PropT F)
+      (k_spec : forall T R, E T -> itree F T -> (T -> itree E R) -> (T -> itree F R) -> itree F R -> Prop)
+      (r : R)
+    , Eq1_PropT _ (interp_prop h_spec k_spec R eq (ret r)) (ret r).
+  Proof.
+    intros.
+    repeat red.
+    split; [| split].
+    - intros. split; intros.
+      + unfold interp_prop in H0.
+        pinversion H0. subst.
+        cbn. rewrite <- H. reflexivity.
+      + pstep. red. do 2 red in H0.
+        rewrite H0 in H.
+
+   (*      rewrite H. eapply Interp_PropT_Ret. cbn. econstructor. reflexivity. rewrite H. cbn in H0. assumption. *)
+   (*  - do 3 red. *)
+   (*    intros t1 t2 eq; split; intros H; pinversion H; subst. *)
+   (*    + red. pstep. econstructor. reflexivity. rewrite <- eq. assumption. *)
+   (*    + red. pstep. econstructor. reflexivity. rewrite eq. assumption. *)
+   (* - do 3 red. intros. split; intros; cbn in *. rewrite <- H. assumption. rewrite H; assumption. *)
+  Admitted.
+
+  #[global] Instance interp_prop_Proper
+   {E F}
+   (h_spec : E ~> PropT F)
+   (k_spec : forall T R, E T -> itree F T -> (T -> itree E R) -> (T -> itree F R) -> itree F R -> Prop)
+   R RR (t : itree E R)
+   (KS: forall A R e ta k1 k2, Proper (eutt eq ==> flip impl) (k_spec A R e ta k1 k2)) :
+    Proper(eq_itree Logic.eq ==> iff) (interp_prop h_spec k_spec R RR t).
+  Proof.
+    do 2 red.
+    intros.
+    split.
+    - revert t x y H.
+      pcofix CIH.
+      intros t x y eq HI.
+      red in HI. punfold HI. red in HI.
+      pstep. red. genobs t ot.
+    (*   inversion HI; subst; econstructor; eauto. *)
+    (*   + rewrite <- eq. assumption. *)
+    (*   + pclearbot. right. eapply CIH; eauto. *)
+    (*   + intros. specialize (HK a H0). pclearbot. right. eapply CIH. 2 : { apply HK. } reflexivity. *)
+    (*   + rewrite <- eq. eauto. *)
+    (* - revert t x y H. *)
+    (*   pcofix CIH. *)
+    (*   intros t x y eq HI. *)
+    (*   red in HI. punfold HI. red in HI. *)
+    (*   pstep. red. genobs t ot. *)
+    (*   inversion HI; subst; econstructor; eauto. *)
+    (*   + rewrite eq. assumption. *)
+    (*   + pclearbot. right. eapply CIH; eauto. *)
+    (*   + intros. specialize (HK a H0). pclearbot. right. eapply CIH. 2 : { apply HK. } reflexivity. *)
+      (*   + rewrite eq. eauto. *)
+  Admitted.
+
+  #[global] Instance interp_prop_Proper2
+   {E F}
+   (h_spec : E ~> PropT F)
+   (k_spec : forall T R, E T -> itree F T -> (T -> itree E R) -> (T -> itree F R) -> itree F R -> Prop)
+   R RR (t : itree E R)
+   (KS: forall A R e ta k1 k2, Proper (eutt eq ==> flip impl) (k_spec A R e ta k1 k2)) :
+    Proper(eutt Logic.eq ==> iff) (interp_prop h_spec k_spec R RR t).
+  Proof.
+    do 2 red.
+    intros.
+    split.
+    - revert t x y H.
+      pcofix CIH.
+      intros t x y eq HI.
+      red in HI. punfold HI. red in HI.
+      pstep. red. genobs t ot.
+    (*   inversion HI; subst; econstructor; eauto. *)
+    (*   + rewrite <- eq. assumption. *)
+    (*   + pclearbot. right. eapply CIH; eauto. *)
+    (*   + intros. specialize (HK a H0). pclearbot. right. eapply CIH. 2 : { apply HK. } reflexivity. *)
+    (*   + rewrite <- eq. eauto. *)
+    (* - revert t x y H. *)
+    (*   pcofix CIH. *)
+    (*   intros t x y eq HI. *)
+    (*   red in HI. punfold HI. red in HI. *)
+    (*   pstep. red. genobs t ot. *)
+    (*   inversion HI; subst; econstructor; eauto. *)
+    (*   + rewrite eq. assumption. *)
+    (*   + pclearbot. right. eapply CIH; eauto. *)
+    (*   + intros. specialize (HK a H0). pclearbot. right. eapply CIH. 2 : { apply HK. } reflexivity. *)
+      (*   + rewrite eq. eauto. *)
+  Admitted.
+
+  (* TODO: Move this *)
+  Lemma eqit_flip_symmetric {E R} (RR : R -> R -> Prop) `{Symmetric R RR} b1 b2:
+    forall (u : itree E R) (v : itree E R),
+      eqit RR b1 b2 u v -> eqit (flip RR) b1 b2 u v.
+  Proof.
+    pcofix self; pstep. intros u v euv. punfold euv.
+    red in euv |- *. induction euv; pclearbot; eauto 7 with paco.
+  Qed.
+
+  #[global] Instance interp_prop_Proper3
+   {E F} {a b}
+   (h_spec : E ~> PropT F)
+   (k_spec : forall T R, E T -> itree F T -> (T -> itree E R) -> (T -> itree F R) -> itree F R -> Prop)
+   (KP : forall T R RR b a, Proper (eq ==> eq ==> (fun k1 k2 => forall x, eqit RR b a (k1 x) (k2 x)) ==> eq ==> eq ==> iff) (k_spec T R))
+   R RR :
+    Proper(eqit eq a b ==> eq  ==> iff) (interp_prop h_spec k_spec R RR).
+  Proof.
+    do 4 red.
+    intros; split.
+    - subst.
+      revert x y H y0.
+      pcofix CIH.
+      intros x y eq t H.
+      pstep; red.
+      punfold H. red in H.
+
+      punfold eq. red in eq.
+      genobs x obsx.
+      genobs y obsy.
+      revert x y Heqobsx Heqobsy t H.
+
+      induction eq; intros x y Heqobsx Heqobsy t H; inversion H; subst; pclearbot.
+      + econstructor; eauto.
+      + econstructor. right. eapply CIH. apply REL. apply HS.
+   (*    + apply inj_pair2 in H2. *)
+   (*      apply inj_pair2 in H3. subst. *)
+   (*      econstructor; eauto. intros X HX. specialize (REL X). specialize (HK X HX). pclearbot. *)
+   (*      right. *)
+
+   (*      eapply CIH; eauto. *)
+   (*      eapply KP; eauto. *)
+   (*      intros. *)
+   (*      eapply eqit_flip; *)
+   (*      eapply eqit_flip_symmetric; eauto; typeclasses eauto. *)
+   (*    + eapply IHeq.  reflexivity. reflexivity. *)
+   (*      punfold HS. *)
+   (*    + econstructor. left. pstep. eapply IHeq. reflexivity. reflexivity. assumption. *)
+   (*    + econstructor. left.  pstep. eapply IHeq. reflexivity. reflexivity. assumption. *)
+   (*    + econstructor. left.  pstep. eapply IHeq. reflexivity. reflexivity. assumption. *)
+
+   (* - subst. *)
+   (*    revert x y H y0. *)
+   (*    pcofix CIH. *)
+   (*    intros x y eq t H. *)
+   (*    pstep; red. *)
+   (*    punfold H. red in H. *)
+
+   (*    punfold eq. red in eq. *)
+   (*    genobs x obsx. *)
+   (*    genobs y obsy. *)
+   (*    revert x y Heqobsx Heqobsy t H. *)
+
+   (*    induction eq; intros x y Heqobsx Heqobsy t H; inversion H; subst; pclearbot. *)
+   (*    + econstructor; eauto. *)
+   (*    + econstructor. right. eapply CIH. apply REL. apply HS. *)
+   (*    + apply inj_pair2 in H2. *)
+   (*      apply inj_pair2 in H3. subst. *)
+   (*      econstructor; eauto. intros X HX. specialize (REL X). specialize (HK X HX). pclearbot. *)
+   (*      right. *)
+
+   (*      eapply CIH; eauto. *)
+   (*      eapply KP; eauto. *)
+   (*    + econstructor. left. pstep. eapply IHeq. reflexivity. reflexivity. assumption. *)
+   (*    + econstructor. left. pstep. eapply IHeq. reflexivity. reflexivity. assumption. *)
+   (*    + econstructor. left. pstep. eapply IHeq. reflexivity. reflexivity. assumption. *)
+        (*    + eapply IHeq. reflexivity. reflexivity.   punfold HS. *)
+  Admitted.
+
+    Lemma interp_prop_ret_pure :
+      forall {T E F} (RR : relation T) `{REF: Reflexive _ RR} (x : T)
+        (h : E ~> PropT F)
+        (k_spec : forall T R, E T -> itree F T -> (T -> itree E R) -> (T -> itree F R) -> itree F R -> Prop),
+      interp_prop h k_spec _ RR (ret x) (ret x).
+    Proof.
+      intros T E F RR REF x h k_spec.
+      generalize dependent x.
+      pcofix CIH.
+      intros x.
+      pstep.
+      cbn.
+      econstructor.
+      reflexivity.
+    Qed.
+ 
+    Lemma interp_prop_ret_refine :
+      forall {T E F} (RR : relation T) (x y : T)
+        (h : E ~> PropT F)
+        (k_spec : forall T R, E T -> itree F T -> (T -> itree E R) -> (T -> itree F R) -> itree F R -> Prop),
+        RR x y ->
+        interp_prop h k_spec _ RR (ret x) (ret y).
+    Proof.
+      intros T E F RR x y h k_spec RRxy.
+      generalize dependent y.
+      generalize dependent x.
+      pcofix CIH.
+      intros x y RRxy.
+      pstep.
+      cbn.
+      econstructor; eauto.
+    Qed.
+
+    Lemma interp_prop_refl_h :
+      forall {T E} (RR : relation T) `{REF: Reflexive _ RR} (t1 t2 : itree E T)
+        (h : E ~> PropT E)
+        (k_spec : forall T R, E T -> itree E T -> (T -> itree E R) -> (T -> itree E R) -> itree E R -> Prop),
+        (forall {X : Type} (e : E X), h X e (trigger e)) ->
+        (k_spec_correct (fun T e => trigger e) k_spec) ->
+        t1 ≈ t2 ->
+        interp_prop h k_spec _ RR t1 t2.
+    Proof.
+      intros T E RR REF t1 t2 h k_spec H_SPEC K_SPEC EQ.
+      generalize dependent t2.
+      generalize dependent t1.
+      pcofix CIH.
+      intros t1 t2 EQ.
+      pose proof (itree_eta t1) as ETA.
+      destruct (observe t1) eqn:Ht1.
+      - pstep.
+        red.
+        rewrite Ht1.
+      (*   econstructor. *)
+      (*   reflexivity. *)
+      (*   rewrite <- EQ. *)
+      (*   rewrite ETA. *)
+      (*   reflexivity. *)
+      (* - pstep. *)
+      (*   red. *)
+      (*   rewrite Ht1. *)
+      (*   econstructor. *)
+      (*   right. *)
+      (*   apply CIH; auto. *)
+      (*   rewrite <- tau_eutt. *)
+      (*   rewrite <- ETA. *)
+      (*   auto. *)
+      (* - pstep. *)
+      (*   red. *)
+      (*   rewrite Ht1. *)
+      (*   eapply Interp_PropT_Vis with (k2 := k). *)
+      (*   + eauto. *)
+      (*   + intros a RET. *)
+      (*     right. *)
+      (*     apply CIH. *)
+      (*     reflexivity. *)
+      (*   + eapply K_SPEC. rewrite <- EQ. *)
+      (*     setoid_rewrite bind_trigger. *)
+      (*     cbn. *)
+      (*     rewrite ETA. *)
+        (*     reflexivity. *)
+    Admitted.
+
+    Lemma interp_prop_refl :
+      forall {T E} (RR : relation T) `{REF: Reflexive _ RR} (t : itree E T)
+        (h : forall X : Type, E X -> PropT E X)
+        (k_spec : forall T R, E T -> itree E T -> (T -> itree E R) -> (T -> itree E R) -> itree E R -> Prop),
+        (forall {X : Type} (e : E X), h X e (trigger e)) ->
+        (k_spec_correct (fun T e => trigger e) k_spec) ->
+        interp_prop h k_spec _ RR t t.
+    Proof.
+      intros T E RR REF t h k_spec H_SPEC K_SPEC.
+      apply interp_prop_refl_h; eauto.
+      reflexivity.
+    Qed.
+
+  (* Lemma 5.4: interp_prop_correct - note that the paper presents a slightly simpler formulation where t = t' *)
+  Lemma interp_prop_correct_exec:
+    forall {E F}
+      (h_spec : E ~> PropT F)
+      (k_spec : forall T R, E T -> itree F T -> (T -> itree E R) -> (T -> itree F R) -> itree F R -> Prop)
+      (h: E ~> itree F)
+      (HC : handler_correct h_spec h)
+      (KC : k_spec_correct h k_spec),
+      forall R RR `{Reflexive _ RR} t t', t ≈ t' -> interp_prop h_spec k_spec R RR t (interp h t').
+  Proof.
+    intros E F h_spec k_spec h HC KC R RR H t t' H1.
+    revert t t' H1.
+    pcofix CIH.
+    intros t t' eq.
+    pstep.
+    red.
+    unfold interp, Basics.iter, MonadIter_itree.
+    rewrite (itree_eta t) in eq.
+    destruct (observe t).
+    (* - econstructor. reflexivity. rewrite <- eq. rewrite unfold_iter. cbn. rewrite Eq.bind_ret_l. cbn.  reflexivity. *)
+    (* - econstructor. right. *)
+    (*   eapply CIH. rewrite tau_eutt in eq. rewrite eq. reflexivity. *)
+    (* - econstructor. *)
+    (*   apply HC. *)
+    (*   intros a. cbn.   *)
+    (*   right. *)
+    (*   unfold interp, Basics.iter, MonadIter_itree in CIH. unfold fmap, Functor_itree, ITree.map in CIH. *)
+    (*   specialize (CIH (k a) (k a)). *)
+    (*   apply CIH. *)
+    (*   reflexivity. *)
+
+    (*   unfold k_spec_correct in KC. *)
+      
+    (*   eapply KC. *)
+    (*   rewrite <- eq. *)
+    (*   rewrite unfold_iter. *)
+    (*   cbn. *)
+
+    (*   rewrite bind_map. *)
+    (*   eapply eutt_clo_bind. *)
+    (*   reflexivity. *)
+    (*   intros u1 u2 H0; subst. *)
+
+    (*   rewrite tau_eutt. *)
+    (*   reflexivity. *)
+  Admitted.
+
+  (* Lemma 5.5 - note that the paper presents this lemma after unfolding the definition of Proper.
+   *)
+  Instance interp_prop_Proper_eq :
+    forall R (RR : relation R) (HR: Reflexive RR) (HT : Transitive RR) E F
+      (h_spec : E ~> PropT F)
+      (k_spec : forall T R, E T -> itree F T -> (T -> itree E R) -> (T -> itree F R) -> itree F R -> Prop)
+      (KP : forall T R RR b a, Proper (eq ==> eq ==> (fun k1 k2 => forall x, eqit RR b a (k1 x) (k2 x)) ==> eq ==> eq ==> iff) (k_spec T R)),
+      Proper (@eutt _ _ _ RR ==> eq ==> flip Basics.impl) (@interp_prop E _ h_spec k_spec R RR).
+  Proof.
+    intros.
+
+    do 5 red.
+    intros t1 t2 eqt s' s eqs HI.
+    subst.
+
+    revert t1 t2 eqt s HI.
+
+    pcofix CIH.
+
+    intros.
+
+    pstep. red.
+    punfold HI. red in HI.
+
+    punfold eqt. red in eqt.
+    genobs t1 obst1.
+    genobs t2 obst2.
+    revert t1 t2 Heqobst1 Heqobst2 s HI.
+
+    induction eqt; intros.
+    - inversion HI; subst.
+      econstructor. etransitivity; eauto.
+    (*   assumption. *)
+    (* - inversion HI; subst. *)
+    (*   econstructor. pclearbot. right.  eapply CIH; eauto. *)
+    (* - inversion HI. *)
+    (*   subst. *)
+    (*   apply inj_pair2 in H1. *)
+    (*   apply inj_pair2 in H2. *)
+    (*   subst. *)
+    (*   econstructor. *)
+    (*   apply HTA. *)
+    (*   intros a Ha. specialize (REL a). specialize (HK a Ha). red in REL. pclearbot. *)
+    (*   right. eapply CIH. apply REL. apply HK. *)
+    (*   eapply KP; eauto. *)
+    (*   pclearbot. *)
+    (*   intros x. *)
+    (*   eapply REL. *)
+    (* - econstructor. *)
+    (*   left. pstep. red. eapply IHeqt. reflexivity. eassumption. assumption. *)
+    (* - inversion HI; subst. *)
+    (*   pclearbot. *)
+    (*   eapply IHeqt. reflexivity. reflexivity. *)
+    (*   pinversion HS. *)
+      Admitted.
+  (* Qed. *)
+
+    Lemma interp_prop_trans :
+      forall {T E} (RR : relation T) `{REF: Reflexive _ RR} `{TRANS: Transitive _ RR} (x y z : itree E T)
+        (h : forall X : Type, E X -> PropT E X)
+        (k_spec : forall T R, E T -> itree E T -> (T -> itree E R) -> (T -> itree E R) -> itree E R -> Prop),
+        (forall {X : Type} (e : E X), h X e (trigger e)) ->
+        (k_spec_correct (fun T e => trigger e) k_spec) ->
+        interp_prop h k_spec _ RR x y ->
+        interp_prop h k_spec _ RR y z ->
+        interp_prop h k_spec _ RR x z.
+    Proof.
+      intros T E RR REF TRANS x y z h k_spec H_SPEC K_SPEC XY YZ.
+      revert x y z XY YZ.
+      pcofix CIH; intros x y z XY YZ.
+
+      punfold XY; punfold YZ; pfold; red in XY, YZ |- *.
+      genobs x xo.
+      genobs y yo.
+      genobs z zo.
+    Abort.
+
+
+  (* Figure 7: interp Trigger law *)
+  (* morally, we should only work with "proper" triggers everywhere *)
+  (* Lemma interp_prop_trigger : *)
+  (*   forall E F *)
+  (*     (h_spec : E ~> PropT F) *)
+  (*     R (e : E R) *)
+  (*     (HP : forall T R k t2, Proper (eq ==> Eq1_PropT T) (fun e ift => h_spec T R e ift k t2)) *)
+  (*   , (forall k t2, Eq1_PropT _ (interp_prop h_spec k_spec R eq (trigger e)) (fun ifr => h_spec R R R e ifr k t2)). *)
+  (* Proof. *)
+  (*   intros. *)
+  (*   red. *)
+  (*   split; [| split]. *)
+  (*   - intros; split; intros. *)
+  (*     + unfold trigger in H0. red in H0. *)
+  (*       pinversion H0; subst. *)
+  (*       apply inj_pair2 in H3. apply inj_pair2 in H4. *)
+  (*       subst. *)
+  (*       unfold subevent, resum, ReSum_id, Id_IFun, id_ in HTA. *)
+  (*       rewrite eq2 in H. *)
+  (*       assert (x <- ta ;; k2 x ≈ ta). *)
+  (*       { rewrite <- (Eq.bind_ret_r ta). *)
+  (*         apply eutt_clo_bind with (UU := fun u1 u2 => u1 = u2 /\ Returns u1 ta). *)
+  (*         rewrite Eq.bind_ret_r. apply eutt_Returns. *)
+  (*         intros. destruct H1. subst. specialize (HK u2 H2). pclearbot. pinversion HK. subst. assumption. *)
+  (*       } *)
+  (*       rewrite H1 in H. *)
+  (*       specialize (HP R e e eq_refl).  unfold Eq1_PropT in HP. destruct HP as (P & _ & _). *)
+  (*       rewrite P. apply HTA. symmetry. assumption. *)
+  (*     + unfold trigger, subevent, resum, ReSum_id, Id_IFun, id_. *)
+  (*       red. pstep. eapply Interp_PropT_Vis with (k2 := (fun x : R => Ret x)). *)
+  (*       * apply H0. *)
+  (*       * unfold bind, Monad_itree. rewrite Eq.bind_ret_r. assumption. *)
+  (*       * intros a. left. pstep. red. econstructor. reflexivity.  reflexivity. *)
+  (*   - do 4 red. intros; split; intros. *)
+  (*     rewrite <- H. assumption. *)
+  (*     rewrite H. assumption. *)
+  (*   - do 4 red. *)
+  (*     intros; split; intros. *)
+  (*     specialize (HP R e e eq_refl). destruct HP as (P & _ & _). *)
+  (*     rewrite P; eauto. symmetry. assumption. *)
+  (*     specialize (HP R e e eq_refl). destruct HP as (P & _ & _). *)
+  (*     rewrite P; eauto.  *)
+  (* Qed. *)
+
+  (* Figure 7: Structural law for tau *)
+  Lemma interp_prop_tau :
+    forall E F
+      (h_spec : E ~> PropT F)
+      (k_spec : forall T R, E T -> itree F T -> (T -> itree E R) -> (T -> itree F R) -> itree F R -> Prop)
+      R RR
+      (t_spec : itree E R)
+      (KP : forall T R e t k1 k2, Proper (eutt eq ==> flip impl) (k_spec T R e t k1 k2)),
+      Eq1_PropT _ (interp_prop h_spec k_spec R RR t_spec) (interp_prop h_spec k_spec R RR (Tau t_spec)).
+  Proof.
+    intros.
+    split; [| split].
+    - intros; split; intros.
+      + rewrite <- H.
+        pstep. red. econstructor.
+    (*     left. *)
+    (*     apply H0. *)
+    (*   + rewrite H. *)
+    (*     pinversion H0. subst. *)
+    (*     apply HS. *)
+    (* - red. typeclasses eauto. *)
+        (* - red. typeclasses eauto. *)
+  Admitted.
+
+  Lemma interp_prop_ret_inv :
+    forall E F
+      (h_spec : E ~> PropT F)
+      (k_spec : forall T R, E T -> itree F T -> (T -> itree E R) -> (T -> itree F R) -> itree F R -> Prop)
+      R RR
+      (r1 : R)
+      (t : itree F R)
+      (H : interp_prop h_spec k_spec R RR (ret r1) t),
+       exists  r2, RR r1 r2 /\ t ≈ ret r2.
+  Proof.
+    intros.
+    punfold H.
+    red in H. inversion H; subst.
+    exists r2; eauto.
+  Admitted.
+
+  Lemma interp_prop_vis_inv :
+    forall E F
+      (h_spec : E ~> PropT F)
+      (k_spec : forall T R, E T -> itree F T -> (T -> itree E R) -> (T -> itree F R) -> itree F R -> Prop)
+      R RR S
+      (e : E S)
+      (k : S -> itree E R)
+      (t : itree F R)
+      (H : interp_prop h_spec k_spec R RR (vis e k) t), 
+    exists  ms, exists (ks : S -> itree F R),
+      h_spec S e ms /\ k_spec S R e ms k ks t.
+  Proof.
+    intros.
+    punfold H.
+    red in H. inversion H; subst.
+    apply inj_pair2 in H2.
+    apply inj_pair2 in H3.
+    subst.
+    exists ta. exists k2. auto.
+  Qed.
+
+  Lemma interp_prop_tau_inv :
+    forall E F
+      (h_spec : E ~> PropT F)
+      (k_spec : forall T R, E T -> itree F T -> (T -> itree E R) -> (T -> itree F R) -> itree F R -> Prop)
+      R RR 
+      (s : itree E R)
+      (t : itree F R)
+      (H : interp_prop h_spec k_spec R RR (Tau s) t), 
+      interp_prop h_spec k_spec R RR s t.
+  Proof.
+    intros.
+    punfold H.
+    red in H. inversion H; subst.
+    pclearbot.
+    (* apply HS. *)
+  Admitted.
+  (* Qed. *)
+
+End interp_prop.
